Feat rust support general trait boxing (#5940)
### Description
- Support for general traits in the Rust backend by compiling them to
boxed dynamic types
- PartialCmp comparison methods like "ab.le(c)" were ambiguous for the
Rust compiler, so added explicit calling code for them

### Refactorings/enhancements
- Conversions require an environment to know the type of identifiers, in
case we need to know their ownership
- Refactored the code of Expression.Call() and Statement.Call() in the
same expression
- Found a simpler termination proof that no longer requires axioms.
- Uncompilable code is no longer unparsable, so that all issues are
resolution errors.
- TokenToString to identify in the generated source code the Dafny code
that is still not compilable
- Removed where clauses in implementations as we did not use them
anymore.
- Removed OwnershipBox as it's no longer a used ownership - will maybe
reintroduce later when we will have custom ownership models.
- Moved the deletion of GeneratedOutputFromDafny-rs.dtr in the python
script so that this step can be called from the IDE.
- 
 
### How has this been tested?
<!-- Tests can be added to
`Source/IntegrationTests/TestFiles/LitTests/LitTest/` or to
`Source/*.Test/…` and run with `dotnet test` -->

<small>By submitting this pull request, I confirm that my contribution
is made under the terms of the [MIT
license](https://github.com/dafny-lang/dafny/blob/master/LICENSE.txt).</small>

Source/DafnyCore/Backends/Dafny/ASTBuilder.cs
@@ -41,12 +41,12 @@ namespace Microsoft.Dafny.Compilers {
 
     public static Module UnsupportedToModule(string why) {
       return new Module(
-        Sequence<Rune>.UnicodeFromString(why.Replace(".", ",")),
+        Sequence<Rune>.UnicodeFromString($"uncompilable/*{why.Replace(".", ",")}*/"),
         Sequence<Attribute>.FromElements(
           (Attribute)Attribute.create_Attribute(
             Sequence<Rune>.UnicodeFromString("extern"),
           Sequence<Sequence<Rune>>.FromElements(
-            (Sequence<Rune>)Sequence<Rune>.UnicodeFromString(why)))), false,
+            (Sequence<Rune>)Sequence<Rune>.UnicodeFromString($"uncompilable/*{why}*/")))), false,
         Std.Wrappers.Option<Sequence<ModuleItem>>.create_None());
     }
   }
@@ -159,8 +159,9 @@ namespace Microsoft.Dafny.Compilers {
   interface TraitContainer : Container {
     void AddTrait(Trait item);
 
-    public TraitBuilder Trait(string name, List<DAST.TypeArgDecl> typeParams, List<DAST.Type> parents, ISequence<_IAttribute> attributes) {
-      return new TraitBuilder(this, name, typeParams, parents, attributes);
+    public TraitBuilder Trait(string name, List<TypeArgDecl> typeParams, List<DAST.Type> parents,
+      ISequence<_IAttribute> attributes, _ITraitType traitType) {
+      return new TraitBuilder(this, name, typeParams, parents, attributes, traitType);
     }
   }
 
@@ -171,12 +172,14 @@ namespace Microsoft.Dafny.Compilers {
     private readonly List<DAST.Type> parents;
     readonly List<DAST.Method> body = new();
     private ISequence<_IAttribute> attributes;
+    private _ITraitType traitType;
 
-    public TraitBuilder(TraitContainer parent, string name, List<DAST.TypeArgDecl> typeParams, List<DAST.Type> parents, ISequence<_IAttribute> attributes) {
+    public TraitBuilder(TraitContainer parent, string name, List<DAST.TypeArgDecl> typeParams, List<DAST.Type> parents, ISequence<_IAttribute> attributes, _ITraitType traitType) {
       this.parent = parent;
       this.name = name;
       this.typeParams = typeParams;
       this.attributes = attributes;
+      this.traitType = traitType;
       this.parents = parents;
     }
 
@@ -200,6 +203,7 @@ namespace Microsoft.Dafny.Compilers {
       parent.AddTrait((Trait)Trait.create(
         Sequence<Rune>.UnicodeFromString(this.name),
         Sequence<DAST.TypeArgDecl>.FromArray(typeParams.ToArray()),
+        traitType,
         Sequence<DAST.Type>.FromArray(parents.ToArray()),
         Sequence<DAST.Method>.FromArray(body.ToArray()),
         attributes)
@@ -321,9 +325,9 @@ namespace Microsoft.Dafny.Compilers {
   interface DatatypeContainer : Container {
     void AddDatatype(Datatype item);
 
-    public DatatypeBuilder Datatype(string name, string enclosingModule, List<DAST.TypeArgDecl> typeParams,
-      List<DAST.DatatypeCtor> ctors, bool isCo, ISequence<_IAttribute> attributes) {
-      return new DatatypeBuilder(this, name, enclosingModule, typeParams, ctors, isCo, attributes);
+    public DatatypeBuilder Datatype(string name, string enclosingModule, List<TypeArgDecl> typeParams,
+      List<DAST.DatatypeCtor> ctors, bool isCo, ISequence<_IAttribute> attributes, List<DAST.Type> superTraitTypes) {
+      return new DatatypeBuilder(this, name, enclosingModule, typeParams, ctors, isCo, attributes, superTraitTypes);
     }
   }
 
@@ -336,8 +340,9 @@ namespace Microsoft.Dafny.Compilers {
     readonly bool isCo;
     readonly List<DAST.Method> body = new();
     private ISequence<_IAttribute> attributes;
+    private List<DAST.Type> superTraitTypes;
 
-    public DatatypeBuilder(DatatypeContainer parent, string name, string enclosingModule, List<DAST.TypeArgDecl> typeParams, List<DAST.DatatypeCtor> ctors, bool isCo, ISequence<_IAttribute> attributes) {
+    public DatatypeBuilder(DatatypeContainer parent, string name, string enclosingModule, List<DAST.TypeArgDecl> typeParams, List<DAST.DatatypeCtor> ctors, bool isCo, ISequence<_IAttribute> attributes, List<DAST.Type> superTraitTypes) {
       this.parent = parent;
       this.name = name;
       this.typeParams = typeParams;
@@ -345,6 +350,7 @@ namespace Microsoft.Dafny.Compilers {
       this.ctors = ctors;
       this.isCo = isCo;
       this.attributes = attributes;
+      this.superTraitTypes = superTraitTypes;
     }
 
     public void AddMethod(DAST.Method item) {
@@ -362,7 +368,8 @@ namespace Microsoft.Dafny.Compilers {
         Sequence<DAST.TypeArgDecl>.FromArray(typeParams.ToArray()),
         Sequence<DAST.DatatypeCtor>.FromArray(ctors.ToArray()),
         Sequence<DAST.Method>.FromArray(body.ToArray()),
-        this.isCo, attributes
+        this.isCo, attributes,
+        Sequence<DAST.Type>.FromArray(superTraitTypes.ToArray())
       ));
       return parent;
     }
@@ -1021,7 +1028,7 @@ namespace Microsoft.Dafny.Compilers {
 
     public void AddBuildable(BuildableExpr value) {
       if (this.value != null) {
-        throw new InvalidOperationException();
+        AddUnsupported("Second value for ReturnBuilder");
       } else {
         this.value = value;
       }
@@ -1316,7 +1323,7 @@ namespace Microsoft.Dafny.Compilers {
 
     static DAST.Expression UnsupportedToExpr(string why) {
       return (DAST.Expression)DAST.Expression.create_Ident(
-        Sequence<ISequence<Rune>>.UnicodeFromString($"<i>Unsupported: {why}</i>")
+        Sequence<ISequence<Rune>>.UnicodeFromString($"uncompilable(\"<i>Unsupported: {why}</i>\")")
       );
     }
   }
